added validity axiom in CData, proved in in RegsData

rocq/RegsData.v
@@ -97,6 +97,15 @@ Module Array.
         lia.
   Qed.
 
+  Lemma zipWith_length {A} {B} {C} : forall (a : t A) (b : t B) (f : (A * B) -> C),
+      length (zipWith a b f) = min (length a) (length b).
+  Proof.
+    intros.
+    unfold zipWith.
+    rewrite length_map.
+    apply length_combine.
+  Qed.
+
 End Array.
 
 
@@ -155,6 +164,18 @@ Module RegsData : CDATA.
         end
     end.
 
+  Fixpoint add_list_to_array (l: list (nat * val))
+    (a: Array.t val) : (Array.t val) :=
+    match l with
+    | [] => a
+    | (i, e) :: l' =>
+        let a' := add_list_to_array l' a in
+        match e with
+        | None => a'
+        | Some v => Array.set a' i e
+        end
+    end.
+
   (* array is more recent than list
    only add list elem if what what there before is None *)
   Fixpoint add_arrays_to_list (l: list (nat * val * val))
@@ -174,8 +195,22 @@ Module RegsData : CDATA.
         add_arrays_to_list l' a_cp' a_clk'
     end.
 
+  Fixpoint add_array_to_list (l: list (nat * val))
+    (a: Array.t val) : (Array.t val) :=
+    match l with
+    | [] => a
+    | (i, e) :: l' =>
+        (* add e to arrays if what is already there is None *)
+        let a' :=
+          match Array.get a i with
+          | Some None => Array.set a i e
+          | _ => a
+          end in
+        add_array_to_list l' a'
+    end.
+
   (* t1 is old, t2 is recent *)
-  Definition compress (p: p) (t1: t) (t2: t): t :=
+  Definition compress' (p: p) (t1: t) (t2: t): t :=
     match t1, t2 with
     | Complete a_cp1 a_clk1, Complete a_cp2 a_clk2 =>
         Complete (merge_arrays a_cp1 a_cp2) (merge_arrays a_clk1 a_clk2)
@@ -187,13 +222,107 @@ Module RegsData : CDATA.
         Complete a_cp a_clk
     | Incomplete l1, Incomplete l2 =>
         let l := l2 ++ l1 in
-        if Nat.leb (length l) p
+        if Nat.leb p (length l)
         then
           let (a_cp, a_clk) := add_list_to_arrays l (Array.make p None) (Array.make p None) in
           Complete a_cp a_clk
         else Incomplete l
     end.
 
+  Definition all_to_cp (x : nat * val * val) : (nat * val) :=
+    match x with
+    | (i, cp, _) => (i, cp)
+    end.
+
+  Definition all_to_clk (x : nat * val * val) : (nat * val) :=
+    match x with
+    | (i, _, clk) => (i, clk)
+    end.
+
+  Definition compress (p: p) (t1: t) (t2: t): t :=
+    match t1, t2 with
+    | Complete a_cp1 a_clk1, Complete a_cp2 a_clk2 =>
+        Complete (merge_arrays a_cp1 a_cp2) (merge_arrays a_clk1 a_clk2)
+    | Complete a_cp1 a_clk1, Incomplete l2 =>
+        let a_cp := add_list_to_array (map all_to_cp l2) a_cp1 in
+        let a_clk := add_list_to_array (map all_to_clk l2) a_clk1 in
+        Complete a_cp a_clk
+    | Incomplete l1, Complete a_cp2 a_clk2 =>
+        let a_cp := add_array_to_list (map all_to_cp l1) a_cp2 in
+        let a_clk := add_array_to_list (map all_to_clk l1) a_clk2 in
+        Complete a_cp a_clk
+    | Incomplete l1, Incomplete l2 =>
+        let l := l2 ++ l1 in
+        if Nat.leb p (length l)
+        then
+          let a_cp := add_list_to_array (map all_to_cp l) (Array.make p None) in
+          let a_clk := add_list_to_array (map all_to_clk l) (Array.make p None) in
+          Complete a_cp a_clk
+        else Incomplete l
+    end.
+  
+  Lemma merge_arrays_length : forall a b,
+      Array.length (merge_arrays a b) = min (Array.length a) (Array.length b).
+  Proof.
+    intros a b.
+    unfold merge_arrays.
+    apply Array.zipWith_length.
+  Qed.
+
+  Lemma add_list_to_array_length : forall l a,
+      Array.length a = Array.length (add_list_to_array l a).
+  Proof.
+    intros l a.
+    induction l as [ | [i e] l]; simpl.
+    - reflexivity.
+    - destruct e eqn:E.
+      + rewrite Array.length_set.
+        assumption.
+      + assumption.
+  Qed.
+
+  Lemma add_array_to_list_length : forall l a,
+      Array.length a = Array.length (add_array_to_list l a).
+  Proof.
+    intros l.
+    induction l as [ | [i e] l]; intros a; simpl.
+    - reflexivity.
+    - destruct (Array.get a i) eqn:V.
+      + destruct v eqn:V'.
+        * apply IHl.
+        * rewrite <- IHl.
+          symmetry.
+          apply Array.length_set.
+      + apply IHl.
+  Qed.
+
+  Lemma compress_valid : forall x y p,
+      is_valid p x ->
+      is_valid p y ->
+      is_valid p (compress p x y).
+  Proof.
+    intros x y p Hx Hy.
+    destruct x as [cpx clkx | lx]; destruct y as [cpy clky | ly]; simpl in *.
+    - destruct Hx as [Hcpx Hclkx]. destruct Hy as [Hcpy Hclky].
+      split;
+        rewrite merge_arrays_length;
+        [rewrite Hcpx, Hcpy | rewrite Hclkx, Hclky];
+        lia.
+    - repeat rewrite <- add_list_to_array_length.
+      assumption.
+    - repeat rewrite <- add_array_to_list_length.
+      assumption.
+    - destruct (p <=? length (ly ++ lx)) eqn:L; simpl.
+      + repeat rewrite <- add_list_to_array_length.
+        split; apply Array.length_make.
+      + split.
+        * apply leb_complete_conv in L.
+          assumption.
+        * apply Forall_app.
+          destruct Hx as [_ Hx]. destruct Hy as [_ Hy].
+          split; assumption.
+  Qed.
+      
   Lemma merge_arrays_assoc : forall x y z,
       merge_arrays x (merge_arrays y z) = merge_arrays (merge_arrays x y) z.
   Proof.
